Cpc/TypePreservation/SeqStringRegex.lean
@@ -138,6 +138,7 @@ theorem typeof_value_seq_nth_wrong
     (ss : SmtSeq)
     (n : smt_lit_Int)
     (T : SmtType)
+    (hT : type_inhabited T)
     (hss : __smtx_typeof_seq_value ss = SmtType.Seq T) :
     __smtx_typeof_value (__smtx_seq_nth_wrong M ss n (SmtType.Seq T)) = T := by
   change __smtx_typeof_value
@@ -154,6 +155,7 @@ theorem typeof_value_seq_nth_wrong
         SmtType.Map (SmtType.Seq T) (SmtType.Map SmtType.Int T) :=
     hM smt_lit_oob_seq_nth_id
       (SmtType.Map (SmtType.Seq T) (SmtType.Map SmtType.Int T))
+      (type_inhabited_map (type_inhabited_map hT))
   rcases map_value_canonical
       (A := SmtType.Seq T) (B := SmtType.Map SmtType.Int T) hLookup with ⟨m0, hm0⟩
   rw [hm0]
@@ -1424,6 +1426,7 @@ theorem typeof_value_model_eval_seq_nth
     (hM : model_total_typed M)
     (t1 t2 : SmtTerm)
     (ht : term_has_non_none_type (SmtTerm.Apply (SmtTerm.Apply SmtTerm.seq_nth t1) t2))
+    (hT : type_inhabited (__smtx_typeof (SmtTerm.Apply (SmtTerm.Apply SmtTerm.seq_nth t1) t2)))
     (hpres1 : __smtx_typeof_value (__smtx_model_eval M t1) = __smtx_typeof t1)
     (hpres2 : __smtx_typeof_value (__smtx_model_eval M t2) = __smtx_typeof t2) :
     __smtx_typeof_value (__smtx_model_eval M
@@ -1439,11 +1442,13 @@ theorem typeof_value_model_eval_seq_nth
   unfold __smtx_seq_nth
   have hssTy : __smtx_typeof_seq_value ss = SmtType.Seq T := by
     simpa [hss, h1, __smtx_typeof_value] using hpres1
+  have hT' : type_inhabited T := by
+    simpa [h1, h2, __smtx_typeof, __smtx_typeof_seq_nth] using hT
   have hd :
       __smtx_typeof_value
         (__smtx_seq_nth_wrong M ss n (__smtx_typeof_seq_value ss)) = T := by
     rw [hssTy]
-    exact typeof_value_seq_nth_wrong M hM ss n T hssTy
+    exact typeof_value_seq_nth_wrong M hM ss n T hT' hssTy
   simpa using ssm_seq_nth_typed (ss := ss) (n := n)
     (d := __smtx_seq_nth_wrong M ss n (__smtx_typeof_seq_value ss)) (T := T) hssTy hd
 
